normalizer_eq_stabilizer'

src/orbit/normalizer'.lean
@@ -2,108 +2,77 @@ import orbit.orbit_stabilizer
 
 
 
+namespace mygroup
+
+open classical function set
+open mygroup.subgroup
+open mygroup.group
+variables {G : Type} [group G]
 
 
-def normalizer' [group G] (H : subgroup G) :=
+def normalizer' (H : subgroup G) :=
  stabilizer (conjugation_action) H
  
 
-lemma mem_normalizer'_def [group G] {H : subgroup G} (x : G) :
+lemma mem_normalizer'_def  {H : subgroup G} (x : G) :
   x ∈ normalizer' H ↔ {k : G | ∃ (h : G) (H : h ∈ H), k = x * h * x⁻¹} = H := subgroup.ext'_iff.symm
 
-lemma mem_normalizer'_iff [group G] {H : subgroup G} (x : G):
+lemma mem_normalizer'_iff {H : subgroup G} (x : G):
   x ∈ normalizer' H ↔ ∀ k : G, k ∈ H ↔ x * k * x⁻¹ ∈ H := 
 begin
   rw mem_normalizer'_def,
   split,
   {  intros hx s,
     rw ext_iff at hx,
-    specialize hx s⁻¹,
+    specialize hx (x * s *x⁻¹) ,
     dsimp at hx,
     rw mem_coe' at hx,
-    rw inv_mem_iff at hx,
+    --rw inv_mem_iff at hx,
     rw ← hx,
     clear hx,
+   -- simp only [@inv_eq _ _ s],
     split,
-     {rintro ⟨h, hh, hs⟩,
-      
-      
-      },
-     {sorry} 
+     {rintro hs,
+        use [s, hs] },
+     { rintro ⟨h, hh, hsx⟩,
+       convert hh,
+       apply mul_left_cancel x, 
+       apply mul_right_cancel x⁻¹,
+       assumption
+     } 
     
   },
 
-  {sorry},  
-  /-have test: s⁻¹ ∈ H ,
-   apply H.inv_mem hs,
-  have: x⁻¹ * s * x = w,
-    apply group.mul_left_cancel x,
-    rw ← group.mul_assoc,
-    rw ← group.mul_assoc,
-    rw group.mul_right_inv,
-    rw group.one_mul,
-    apply group.mul_right_cancel x⁻¹,
-    rw group.mul_assoc,
-    rw group.mul_right_inv,
-    rw group.mul_one,
-    assumption,-/
-  
+  {intro hx,
+    ext y,
+    split,
+        {rintro ⟨s, hs, rfl⟩,
+          exact ( hx s ).1 hs},
+        { intro hy,
+          dsimp,
+          use x⁻¹ * y * x,
+          split,
+            {   change y ∈ H at hy,
+                convert (hx (x⁻¹ * y * x)).2 _,
+                convert hy,
+                simp [group.mul_assoc]
+            },
+            {simp [group.mul_assoc]}
+           }
+    },  
 
 
 end  
-
-
-lemma normalizer_eq_stabilizer'' [group G] (H : subgroup G) : 
-(normalizer' H  : set G) = {g : G | ∀ n, n ∈ H ↔ g * n * g⁻¹ ∈ H} := 
-begin
-   ext1,
-   rw subgroup.mem_coe',
-   rw mem_normalizer'_def,
-   rw ext_iff,
-   split,
-   intro h,
-   sorry
-end
-
 
 
 lemma normalizer_eq_stabilizer' [group G] (H : subgroup G) : 
 (normalizer' H  : set G) = {g : G | ∀ n, n ∈ H ↔ g * n * g⁻¹ ∈ H} := 
 begin
    ext1,
-   split,
-    intro hx,
-    dsimp at *,
-    intro n,
-    split, 
-      intro hn,
-      unfold_coes at hx,
-      unfold normalizer' at hx,
-      unfold stabilizer at hx,
-      unfold conjugation_action at hx,
-      unfold conjugate_subgroup at hx,
-      simp at *,
-      rw ← hx,
-      rw ← subgroup.mem_coe,
-      dsimp,
-      use n,
-      split,
-      exact hn,
-      refl,
-
-  intro hxn,
-  unfold_coes at hx,
-  unfold normalizer' at hx,
-  unfold stabilizer at hx,
-  unfold conjugation_action at hx,
-  unfold conjugate_subgroup at hx,
-  simp at *,
-  
-
-      
-  sorry
-
-end  
+   rw subgroup.mem_coe',
+   rw mem_normalizer'_iff,
+   refl,      
+end
 
 
 lemma index_normalizer_congr_index_modp [fintype G]{p : ℕ} (hp: p.prime) (H : subgroup G) (h: is_p_subgroup H p):
@@ -116,3 +85,4 @@ lemma normalizer_neq_subgroup [fintype G](H : subgroup G){p : ℕ}(hp: p.prime)(
 theorem sylow_one_part1 [fintype G] {p m n: ℕ}{hp : p.prime} {hG : fincard' G = p^n * m} {hdiv : ¬ p ∣ m}:
 ∀ (i ≤ n), ∃ (H : subgroup G), fincard' H = p^i := sorry
 -- and want to write that each of these subgroups of cardinality p^i is normal in a subgroup of cardinality p^(i+1)
+end mygroup
