src/orbit/orbit_stabilizer.lean
@@ -696,5 +696,4 @@ begin
 end  -/
 
 
-
 end mygroup
